Rust semantics

Rustv/Rust_Semantics.thy
@@ -2,8 +2,17 @@ theory Rust_Semantics
   imports Rustv Simpl.Vcg
 begin
 
-section \<open>Shallow embedding of Rust Primitives\<close>
+section \<open>Shallow Embedding of Rust Primitives\<close>
 
+subsection \<open>Types\<close>
+datatype rust_integer = ri
+datatype 'a rust_ref = rr
+datatype 'a typed_ref = typed tagged_ref
+
+fun untyped where
+  "untyped (typed r) = r"
+
+subsection \<open>Statements\<close>
 (* In this theory, we are translating Rust assignments of the form of
  * *dst = *src;
  * as follows.
@@ -26,9 +35,28 @@ abbreviation reborrow_stmt where
     Guard invalid_ref {s. writable (from s) s}
       (Basic (\<lambda>s. pop_tags (from s) s);;
       Basic (\<lambda>s. (let (r, s') = reborrow k (from s) s in to s' r)))"
+(* make it stuck if read value is not reference *)
+abbreviation write_imm_typed where
+  "write_imm_typed dst value ==
+    Guard invalid_ref {s. readable (untyped (dst s)) s}
+      (Basic (\<lambda>s. pop_tags (untyped (dst s)) s);;
+      Guard invalid_ref {s. writable (the_ref (memread (untyped (dst s)) s)) s}
+        (Basic (\<lambda>s. pop_tags (the_ref (memread (untyped (dst s)) s)) s);;
+        Basic (\<lambda>s. memwrite (the_ref (memread (untyped (dst s)) s)) value s)))"
+abbreviation reborrow_typed where
+  "reborrow_typed k from to ==
+    Guard invalid_ref {s. writable (untyped (from s)) s \<and> writable (untyped (to s)) s}
+      (Basic (\<lambda>s. pop_tags (untyped (from s)) s);;
+      Basic (\<lambda>s. pop_tags (untyped (to s)) s);;
+      Basic (\<lambda>s. (let (r, s') = reborrow k (untyped (from s)) s in
+            memwrite (untyped (to s')) (ref r) s')))"
+
+subsection \<open>Primitive Expressions\<close>
 
 abbreviation ptr_eq :: "tagged_ref \<Rightarrow> tagged_ref \<Rightarrow> bool" where
   "ptr_eq r1 r2 == the_ptr (pointer r1) = the_ptr (pointer r2)"
+
+subsection \<open>Notations for Control Flow\<close>
 
 syntax
   "_Cond'" :: "'a bexp => ('a,'p,'f) com => ('a,'p,'f) com => ('a,'p,'f) com"
