Rustv/Tests/Rustv_Tests.thy
@@ -2,6 +2,7 @@ theory Rustv_Tests
   imports
     Write
     No_Alias
+    No_Alias_Precise
     SharedWrite
     Cell
     Swap
