Rustv/Tests/ex/No_Alias_Precise.thy
@@ -1,0 +1,49 @@
+theory No_Alias_Precise
+  imports Simpl.Vcg "Rust-Verification.Rust_Semantics"
+begin
+
+record no_alias_env = globals_ram +
+  x :: "rust_integer typed_ref" (* locals are represented by owning reference *)
+  ref1 :: "(rust_integer typed_ref) typed_ref"
+  ref2 :: "(rust_integer typed_ref) typed_ref"
+
+definition no_alias_body :: "(no_alias_env, 'p, rust_error) com" where
+  "no_alias_body ==
+    Basic (\<lambda>s. (let (r, s') = heap_new (int_val 100) s in s'\<lparr> x := typed r \<rparr>));;
+    Basic (\<lambda>s. (let (r, s') = heap_new uninit s in s'\<lparr> ref1 := typed r \<rparr>));;
+    Basic (\<lambda>s. (let (r, s') = heap_new uninit s in s'\<lparr> ref2 := typed r \<rparr>));;
+
+    reborrow_typed Unique x ref1;;
+    write_imm_typed ref1 (int_val 200);;
+
+    reborrow_typed Unique x ref2;;
+    write_imm_typed ref2 (int_val 300)"
+
+lemma suc_len_access[simp]: "length ys \<ge> 2 \<Longrightarrow> (xs @ ys) ! Suc (length xs) = ys ! 1"
+  by (metis Suc_eq_plus1 nth_append_length_plus)
+lemma suc2_len_access[simp]: "length ys \<ge> 3 \<Longrightarrow> (xs @ ys) ! Suc (Suc (length xs)) = ys ! 2"
+  by (metis add_2_eq_Suc' nth_append_length_plus)
+
+(* Termination, by full VCG *)
+lemma "\<Gamma> \<turnstile>\<^sub>t {s. wf_heap s} no_alias_body {s. True}"
+  unfolding no_alias_body_def
+  apply vcg
+  apply (auto simp: Let_def)
+  done
+
+(* Spec of the program *)
+(*
+lemma "\<Gamma> \<turnstile>\<^sub>t
+  {s. wf_heap s}
+  no_alias_body
+  {s. (let p = the_ptr (pointer (untyped (x s))) in
+      memory s ! p = int_val 300) \<and>
+      writable (untyped (x s)) s \<and> \<not>writable (untyped (ref1 s)) s \<and> writable (untyped (ref2 s)) s}"
+  unfolding no_alias_body_def
+  apply vcg
+  (* This auto takes too long because of the term size *)
+  apply (auto simp: Let_def)
+  oops
+*)
+
+end
